Auto/Lib/ListExtra.lean
@@ -123,4 +123,7 @@ theorem List.map_equiv (f₁ f₂ : α → β) (hequiv : ∀ x, f₁ x = f₂ x)
   case cons head tail IH =>
     dsimp [List.map]; rw [hequiv, IH]
 
+theorem List.length_reverseAux (l₁ l₂ : List α) : (l₁.reverseAux l₂).length = l₁.length + l₂.length := by
+  rw [List.reverseAux_eq]; rw [List.length_append]; rw [List.length_reverse]
+
 end Auto
