Auto/Translation/LamFOLization.lean
@@ -1,0 +1,3 @@
+import Lean
+import Auto.Translation.LamReif
+
